Equiv/BisimSim.v
@@ -1,13 +1,13 @@
 Require Import List.
 Require Export Util Var Val Exp Env Map CSet AutoIndTac IL AllInRel Sawtooth.
-Require Export SmallStepRelations StateType Equiv Bisim Sim.
+Require Export SmallStepRelations StateType Bisim Sim.
 
 Set Implicit Arguments.
 Unset Printing Records.
 
-Lemma bisim_sim {S1} `{StateType S1}
+Lemma bisim_sim t {S1} `{StateType S1}
       (σ1:S1) {S2} `{StateType S2} (σ2:S2)
-  : Bisim.bisim σ1 σ2 -> Sim.sim σ1 σ2.
+  : Bisim.bisim σ1 σ2 -> Sim.sim t σ1 σ2.
 Proof.
   revert σ1 σ2. cofix; intros.
   inv H1.
@@ -16,4 +16,17 @@ Proof.
     + intros. edestruct H6; eauto; dcr. eexists; eauto.
     + intros. edestruct H7; eauto; dcr. eexists; eauto.
   - econstructor 4; eauto.
+Qed.
+
+Lemma sim_bisim {S1} `{StateType S1}
+      (σ1:S1) {S2} `{StateType S2} (σ2:S2)
+  : Sim.sim Bisim σ1 σ2 -> Bisim.bisim σ1 σ2.
+Proof.
+  revert σ1 σ2. cofix; intros.
+  inv H1.
+  - econstructor; eauto.
+  - econstructor 2; eauto.
+    + intros. edestruct H6; eauto; dcr. eexists; eauto.
+    + intros. edestruct H7; eauto; dcr. eexists; eauto.
+  - econstructor 3; eauto.
 Qed.
