TrueLiveness.v
@@ -1,5 +1,5 @@
 Require Import AllInRel List Map Env DecSolve.
-Require Import IL Annotation AutoIndTac Bisim Exp MoreExp SetOperations.
+Require Import IL Annotation AutoIndTac Exp MoreExp SetOperations.
 Require Export Liveness Filter LabelsDefined OUnion.
 
 Set Implicit Arguments.
